src/lean4/human_eval/problem_24.lean
@@ -21,9 +21,30 @@ def problem_spec
 let spec (result: Nat) :=
 n > 0 → ∀ x, x ∣ n → x ≠ n → x ≤ result;
 -- program termination
-∃ result, implementation n = result →
+∃ result, implementation n = result ∧
 spec result
 -- end_def problem_spec
+
+-- start_def generated_spec
+def generated_spec
+-- function signature
+(implementation: Nat → Nat)
+-- inputs
+(n: Nat) : Prop :=
+-- end_def generated_spec
+-- start_def generated_spec_body
+sorry
+-- end_def generated_spec_body
+
+-- start_def spec_isomorphism
+theorem spec_isomorphism:
+∀ implementation,
+(∀ n, problem_spec implementation n) ↔
+(∀ n, generated_spec implementation n) :=
+-- end_def spec_isomorphism
+-- start_def spec_isomorphism_proof
+sorry
+-- end_def spec_isomorphism_proof
 
 -- start_def implementation_signature
 def implementation (n: Nat) : Nat :=
