src/lean4/human_eval/problem_34.lean
@@ -22,9 +22,30 @@ let spec (result: List Int) :=
 (∀ x, x ∈ result ↔ x ∈ l ∧ result.count x = 1) ∧
 List.Sorted Int.le result
 -- program termination
-∃ result, implementation l = result →
+∃ result, implementation l = result ∧
 spec result
 -- end_def problem_spec
+
+-- start_def generated_spec
+def generated_spec
+-- function signature
+(implementation: List Int → List Int)
+-- inputs
+(l: List Int) : Prop :=
+-- end_def generated_spec
+-- start_def generated_spec_body
+sorry
+-- end_def generated_spec_body
+
+-- start_def spec_isomorphism
+theorem spec_isomorphism:
+∀ implementation,
+(∀ l, problem_spec implementation l) ↔
+(∀ l, generated_spec implementation l) :=
+-- end_def spec_isomorphism
+-- start_def spec_isomorphism_proof
+sorry
+-- end_def spec_isomorphism_proof
 
 -- start_def implementation_signature
 def implementation (l: List Int) : List Int :=
